Poe.lean
@@ -7,7 +7,7 @@ import Poe.Oracle
 import Poe.Lint
 import Poe.Examples.First
 import Poe.Examples.OutOfFragment
-import Poe.Examples.HelloWorld
+import Poe.Examples.HelloWorldString
 import Poe.Examples.DataDecoding
 import Poe.Examples.AikenHelloWorld
-import Poe.Examples.ScriptContext
+import Poe.Examples.HelloWorld
